First complete version of the evaluator (not tested, not proved).

Basics.v
@@ -1,10 +1,65 @@
-Require Export Arith Program Equations Have.
+Require Export Arith Program Equations Have Morphisms EquivDec.
 
 Hint Extern 4 => discriminates : core.
 
 Ltac simpdep := reverse ; simplify_dep_elim ; simplify_IH_hyps.
 
 Definition ltb (x y : nat) := leb (S x) y.
+
+
+Require Import Relation_Definitions.
+
+Class StrictOrder `(Equivalence A eqA) (ordA : relation A) :=
+  { StrictOrder_trans :> Transitive ordA ;
+    StrictOrder_irrefl :> Irreflexive ordA }.    
+
+Inductive comparison `{E : Equivalence A eqA} ordA `{O : StrictOrder A eqA ordA} (x y : A) : Type :=
+| compare_LT : ordA x y -> comparison ordA x y
+| compare_EQ : eqA x y -> comparison ordA x y 
+| compare_GT : ordA y x -> comparison ordA x y.
+
+Class CompareDec `(E : Equivalence A eqA) `(O : StrictOrder A eqA ordA) :=
+  compare_dec : Π x y : A, comparison ordA x y.
+
+Instance lt_strict_order : ! StrictOrder nat eq lt.
+Proof. constructor ; firstorder. Qed.
+
+Instance nat_compare_dec : ! CompareDec nat eq lt.
+Proof.
+  intros x y. destruct (lt_eq_lt_dec x y) as [ [ lt | eq ] | gt ].
+  now apply compare_LT.
+  now apply compare_EQ.
+  now apply compare_GT.
+Defined.
+
+
+Instance: Proper (le --> le ++> impl) lt.
+Proof. reduce_goal. unfold flip in *. omega. Qed.
+
+Instance: Proper (le --> le ++> impl) le.
+Proof. reduce_goal. unfold flip in *. omega. Qed.
+
+Instance: Proper (le --> lt ++> impl) le.
+Proof. reduce_goal. unfold flip in *. omega. Qed.
+
+Instance: subrelation lt le.
+Proof. reduce_goal. omega. Qed.
+
+Instance: Proper (lt --> lt ++> impl) lt.
+Proof. reduce_goal. unfold flip in *. omega. Qed.
+
+Instance: Proper (le ++> le ++> le) mult.
+Proof. reduce_goal. unfold flip in *. now apply mult_le_compat. Qed.
+
+Program Instance: Reflexive le.
+Program Instance: Transitive le := le_trans.
+Program Instance: PreOrder le.
+
+Lemma mult_lt_compat : Π n m p q : nat, n < m -> p <= q -> q > 0 -> n * p < m * q.
+Proof. intros. induction H. simpl. induction H0 ; try omega. 
+  rewrite H0. ring_simplify. omega.
+  ring_simplify. omega.
+Qed.
 
 Program Fixpoint euclid (n : nat) (m : nat) `{Have (m > 0)} {wf lt n} : nat * nat :=
   match ltb n m with
@@ -51,6 +106,15 @@ Proof.
   omega.
 Defined.
 
+Lemma euclid_unfold n m `{Have (m > 0)} : euclid n m = 
+  if ltb n m then (0, n) else let '(q, r) := euclid (n - m) m in (S q, r).
+Proof.
+  intros. unfold euclid. ind_on euclid_func. admit.
+  destruct x as [ n' [ m' Hm' ] ]; simpl in *.
+  destruct_call ltb. reflexivity.
+  reflexivity.
+Qed.
+
 Eval compute in (euclid 66 8).
 
 Definition quotient_nat n m `{Have (m > 0)} : nat := fst (euclid n m).
@@ -61,3 +125,96 @@ Proof. intros x y H. unfold modulo_nat, quotient_nat in *.
   generalize (euclid_spec x y). destruct_call euclid ; intros Heucl ; simplify_IH_hyps.
   simpl in *. intros. subst. ring.
 Defined.
+
+Lemma euclid_0 y `{Have (y > 0)} : euclid 0 y = (0, 0).
+Proof. intros.
+  generalize (euclid_spec 0 y).
+  destruct_call euclid ; intros ; simplify_IH_hyps.
+  induction n. ring_simplify in H0. subst ; reflexivity.
+  unfold Have in *.
+  destruct y. inversion H.
+  ring_simplify in H0.
+  replace (y * n + y + n + n0 + 1) with (S (y * n + y + n + n0)) in H0 by ring.
+  discriminate.
+Qed.  
+
+Ltac destruct_equiv x y := let Heq := fresh "H" x y in
+  destruct (equiv_dec x y) as [ Heq | Heq ] ; [ try (red in Heq ; subst x) | ].
+
+Lemma modusponens: forall (P Q: Type), P -> (P -> Q) -> Q.
+Proof. auto. Qed.
+
+Ltac exploit x :=
+    refine (modusponens _ _ (x _ _ _ _ _ _ _ _ _ _ _ _ _ _ _ _ _ _ _ _ _ _ _ _ _ _ _ _ _ _ _ _ _ _ _) _)
+ || refine (modusponens _ _ (x _ _ _ _ _ _ _ _ _ _ _ _ _ _ _ _ _ _ _ _ _ _ _ _ _ _ _ _ _ _ _ _ _ _) _)
+ || refine (modusponens _ _ (x _ _ _ _ _ _ _ _ _ _ _ _ _ _ _ _ _ _ _ _ _ _ _ _ _ _ _ _ _ _ _ _ _) _)
+ || refine (modusponens _ _ (x _ _ _ _ _ _ _ _ _ _ _ _ _ _ _ _ _ _ _ _ _ _ _ _ _ _ _ _ _ _ _ _) _)
+ || refine (modusponens _ _ (x _ _ _ _ _ _ _ _ _ _ _ _ _ _ _ _ _ _ _ _ _ _ _ _ _ _ _ _ _ _ _) _)
+ || refine (modusponens _ _ (x _ _ _ _ _ _ _ _ _ _ _ _ _ _ _ _ _ _ _ _ _ _ _ _ _ _ _ _ _ _) _)
+ || refine (modusponens _ _ (x _ _ _ _ _ _ _ _ _ _ _ _ _ _ _ _ _ _ _ _ _ _ _ _ _ _ _ _ _) _)
+ || refine (modusponens _ _ (x _ _ _ _ _ _ _ _ _ _ _ _ _ _ _ _ _ _ _ _ _ _ _ _ _ _ _ _) _)
+ || refine (modusponens _ _ (x _ _ _ _ _ _ _ _ _ _ _ _ _ _ _ _ _ _ _ _ _ _ _ _ _ _ _) _)
+ || refine (modusponens _ _ (x _ _ _ _ _ _ _ _ _ _ _ _ _ _ _ _ _ _ _ _ _ _ _ _ _ _) _)
+ || refine (modusponens _ _ (x _ _ _ _ _ _ _ _ _ _ _ _ _ _ _ _ _ _ _ _ _ _ _ _ _) _)
+ || refine (modusponens _ _ (x _ _ _ _ _ _ _ _ _ _ _ _ _ _ _ _ _ _ _ _ _ _ _ _) _)
+ || refine (modusponens _ _ (x _ _ _ _ _ _ _ _ _ _ _ _ _ _ _ _ _ _ _ _ _ _ _) _)
+ || refine (modusponens _ _ (x _ _ _ _ _ _ _ _ _ _ _ _ _ _ _ _ _ _ _ _ _ _) _)
+ || refine (modusponens _ _ (x _ _ _ _ _ _ _ _ _ _ _ _ _ _ _ _ _ _ _ _ _) _)
+ || refine (modusponens _ _ (x _ _ _ _ _ _ _ _ _ _ _ _ _ _ _ _ _ _ _ _) _)
+ || refine (modusponens _ _ (x _ _ _ _ _ _ _ _ _ _ _ _ _ _ _ _ _ _ _) _)
+ || refine (modusponens _ _ (x _ _ _ _ _ _ _ _ _ _ _ _ _ _ _ _ _ _) _)
+ || refine (modusponens _ _ (x _ _ _ _ _ _ _ _ _ _ _ _ _ _ _ _ _) _)
+ || refine (modusponens _ _ (x _ _ _ _ _ _ _ _ _ _ _ _ _ _ _ _) _)
+ || refine (modusponens _ _ (x _ _ _ _ _ _ _ _ _ _ _ _ _ _ _) _)
+ || refine (modusponens _ _ (x _ _ _ _ _ _ _ _ _ _ _ _ _ _) _)
+ || refine (modusponens _ _ (x _ _ _ _ _ _ _ _ _ _ _ _ _) _)
+ || refine (modusponens _ _ (x _ _ _ _ _ _ _ _ _ _ _ _) _)
+ || refine (modusponens _ _ (x _ _ _ _ _ _ _ _ _ _ _) _)
+ || refine (modusponens _ _ (x _ _ _ _ _ _ _ _ _ _) _)
+ || refine (modusponens _ _ (x _ _ _ _ _ _ _ _ _) _)
+ || refine (modusponens _ _ (x _ _ _ _ _ _ _ _) _)
+ || refine (modusponens _ _ (x _ _ _ _ _ _ _) _)
+ || refine (modusponens _ _ (x _ _ _ _ _ _) _)
+ || refine (modusponens _ _ (x _ _ _ _ _) _)
+ || refine (modusponens _ _ (x _ _ _ _) _)
+ || refine (modusponens _ _ (x _ _ _) _)
+ || refine (modusponens _ _ (x _ _) _)
+ || refine (modusponens _ _ (x _) _).
+
+Tactic Notation "omega" "*" := unfold Have in * ; omega.
+Ltac unhave := unfold Have in *.
+
+Lemma quotient_gt_1 x y `{Have (y > 0)} : x > y -> modulo_nat x y = 0 -> quotient_nat x y > 1.
+Proof. intros x y H. unfold modulo_nat, quotient_nat. generalize (euclid_spec x y).
+  destruct_call euclid ; program_simpl. simplify_IH_hyps. subst x. ring_simplify in H1.
+  unhave. repeat (destruct n; try omega).
+Qed.
+Require Import SetoidTactics.
+
+Lemma plus_minus_le x y : x + y - y = x.
+Proof. induction y.
+  rewrite <- minus_n_O. auto.
+  replace (x + S y) with (S (x + y)) by ring.
+  simpl. apply IHy.
+Qed.
+
+Lemma euclid_mult y `{Have (y > 0)} n : euclid (n * y) y = (n, 0).
+Proof.
+  induction n. 
+    now rewrite euclid_0.
+
+    rewrite euclid_unfold.
+    case_eq (ltb (S n * y) y).
+    intros Hxy; apply leb_complete in Hxy. 
+    replace (S (S n * y)) with (S y + n * y) in Hxy by ring.
+    elimtype False. assert(S y <= S y + n * y) by auto with arith. rewrite <- H0 in Hxy.
+    elim (le_Sn_n _ Hxy).
+
+    intros. apply leb_complete_conv in H0. 
+    replace (S n * y - y) with (n * y). rewrite IHn. reflexivity.
+    simpl. rewrite plus_comm. rewrite plus_minus_le. reflexivity.
+Qed.
+
+Lemma modulo_cancel : forall n y `{Have (y > 0)}, modulo_nat (n * y) y = 0.
+Proof. intros n y H. unfold modulo_nat in *. rewrite euclid_mult. reflexivity. Qed.
+
